src/test/dafny/CallExample.dfy
@@ -1,0 +1,106 @@
+// An set of examples illustrating contract calls.
+include "../../dafny/evm.dfy"
+include "../../dafny/evms/berlin.dfy"
+
+module CallExamples {
+    import opened Int
+    import opened Opcode
+    import opened Memory
+    import EvmBerlin
+    import opened Bytecode
+    import Bytes
+
+    /** The gas loaded in the EVM before executing a program. */
+    const INITGAS := 0xFFFF;
+
+    method test_call_01() {
+        // This is an absolutely minimal example of a contract call where the
+        // called contract just stops.  Since the called contract stopped
+        // successfully, we can at least check the exit code.
+        var vm1 := EvmBerlin.InitEmpty(gas := INITGAS);
+        vm1 := Push1(vm1,0x0); // Out size
+        vm1 := Dup(vm1,1);     // Out offset
+        vm1 := Dup(vm1,1);     // In size
+        vm1 := Dup(vm1,1);     // In offset
+        vm1 := Dup(vm1,1);     // Call value
+        vm1 := Push2(vm1,0xccc); // To address
+        vm1 := Push1(vm1,0x3); // Gas
+        vm1 := Call(vm1);
+        // >>> Contract call starts here
+        {
+            var vm2 := vm1.CallEnter(map[],[]);
+            vm2 := Stop(vm2);
+            vm1 := vm1.CallReturn(vm2);
+        }
+        // <<< Contract call ends here
+        assert vm1.OK?;
+        // Check exit code loaded correctly.
+        assert vm1.Peek(0) == 1;
+    }
+
+    method test_call_02() {
+        // This is another simple example of a contract call where the called
+        // contract raises an exception.
+        var vm1 := EvmBerlin.InitEmpty(gas := INITGAS);
+        vm1 := Push1(vm1,0x0); // Out size
+        vm1 := Dup(vm1,1);     // Out offset
+        vm1 := Dup(vm1,1);     // In size
+        vm1 := Dup(vm1,1);     // In offset
+        vm1 := Dup(vm1,1);     // Call value
+        vm1 := Push2(vm1,0xccc); // To address
+        vm1 := Push1(vm1,0x3); // Gas
+        vm1 := Call(vm1);
+        // >>> Contract call starts here
+        {
+            var vm2 := vm1.CallEnter(map[],[]);
+            vm2 := Pop(vm2); // force exception
+            vm1 := vm1.CallReturn(vm2);
+        }
+        // <<< Contract call ends here
+        assert vm1.OK?;
+        // Check exit code loaded correctly.
+        assert vm1.Peek(0) == 0;
+    }
+
+    method test_call_03() {
+        // This is another simple example of a contract call where the called
+        // contract returns some return data.
+        var vm1 := EvmBerlin.InitEmpty(gas := INITGAS);
+        vm1 := Push1(vm1,0x20);  // Out size
+        vm1 := Push1(vm1,0x0);   // Out offset
+        vm1 := Dup(vm1,1);       // In size
+        vm1 := Dup(vm1,1);       // In offset
+        vm1 := Dup(vm1,1);       // Call value
+        vm1 := Push2(vm1,0xccc); // To address
+        vm1 := Push1(vm1,0xFF);   // Gas
+        vm1 := Call(vm1);
+        { // >>> Contract call starts here
+            var vm2 := vm1.CallEnter(map[],[]);
+            vm2 := contractReturns123(vm2);
+            vm1 := vm1.CallReturn(vm2);
+        } // <<< Contract call ends here
+        // Check exit code loaded correctly.
+        assert vm1.Peek(0) == 1;
+        // Extract return data
+        vm1 := Push1(vm1,0x00);
+        vm1 := MLoad(vm1);
+        // Check return data.
+        assert vm1.Peek(0) == 0x123;
+    }
+
+    method contractReturns123(vm:EvmState.State) returns (vm':EvmState.State)
+    requires vm.OK?
+    requires vm.Capacity() > 3 && vm.MemSize() == 0
+    // Returns exactly 32 bytes of data
+    ensures vm'.RETURNS? && |vm'.data| == 32
+    // Returns exactly 0x123
+    ensures Int.ReadUint256(vm'.data,0) == 0x123 {
+        vm' := vm;
+        vm' := Push2(vm',0x123);
+        vm' := Push1(vm',0x00);
+        vm' := MStore(vm');
+        vm' := Push1(vm',0x20);
+        vm' := Push1(vm',0x00);
+        vm' := Return(vm'); // force return
+    }
+}
